theories/lang/lang_extra.v
@@ -257,40 +257,33 @@ Qed.
     done.
   Qed.
 
-  Lemma transaction_retrieve_descriptor_valid {j handle wf l psd σ} des p :
-    (finz.to_z l) = (Z.of_nat (length psd)) ->
-    des = [of_imm (encode_vmid j); wf; handle; l; of_imm (encode_vmid (get_current_vm σ))] ++ map of_pid psd ->
+  Lemma transaction_retrieve_descriptor_valid {j handle wf σ} des p :
+    des = [of_imm (encode_vmid j); wf; handle; of_imm (encode_vmid (get_current_vm σ))]->
     seq_in_page (of_pid p) (length des) p ->
     (∀ (k : nat) (y1 y2 : Addr),
              finz.seq (of_pid p) (length des) !! k = Some y1 → des !! k = Some y2 → get_mem σ !! y1 = Some y2) ->
     parse_transaction_descriptor_retrieve σ p = Some (j, Some handle, wf, (get_current_vm σ), []).
   Proof.
-    intros H H0 H1 H2.
+    intros H H0 H1.
     rewrite /parse_transaction_descriptor_retrieve /get_memory_with_offset.
-    destruct H1 as [_ [? _]].
-    simpl in H0.
-    pose proof (@trans_desc_length j (get_current_vm σ) wf l psd handle des) as H3.
-    rewrite /serialized_transaction_descriptor /serialized_memory_descirptor in H3.
-    simpl in H3.
-    pose proof (H3 H0) as Hlen.
-    assert (HpSome: ((of_pid p) + 0)%f = Some ((of_pid p) ^+ 0)%f).
+    destruct H0 as [_ [? _]].
+    simpl.
+    pose proof (last_addr_in_bound p) as HSome.
+    assert ( ((of_pid p) + 0)%f = Some ((of_pid p) ^+ 0)%f) as ->.
     solve_finz.
-    rewrite HpSome //=;clear HpSome.
-    rewrite (H2 0 ((of_pid p) ^+ 0)%f (encode_vmid j)).
-    2: { apply finz_seq_lookup. rewrite H0. simpl. lia. solve_finz. }
-    2: { rewrite H0 /serialized_transaction_descriptor. by list_simplifier. }
-    assert (HpSome: ((of_pid p) + 1)%f = Some ((of_pid p) ^+ 1)%f).
+    rewrite (H1 0 ((of_pid p) ^+ 0)%f (encode_vmid j)).
+    2: { apply finz_seq_lookup. rewrite H /=. lia. solve_finz. }
+    2: { rewrite H. by list_simplifier. }
+    assert (((of_pid p) + 1)%f = Some ((of_pid p) ^+ 1)%f) as ->.
     solve_finz.
-    rewrite HpSome //=;clear HpSome.
-    rewrite (H2 1 ((of_pid p) ^+ 1)%f wf).
-    2: { apply finz_seq_lookup. rewrite H0. simpl. lia. solve_finz. }
-    2: { rewrite H0 /serialized_transaction_descriptor. by list_simplifier. }
-    assert (HpSome: ((of_pid p) + 2)%f = Some ((of_pid p) ^+ 2)%f).
+    rewrite (H1 1 ((of_pid p) ^+ 1)%f wf).
+    2: { apply finz_seq_lookup. rewrite H /=. lia. solve_finz. }
+    2: { rewrite H . by list_simplifier. }
+    assert (((of_pid p) + 2)%f = Some ((of_pid p) ^+ 2)%f) as ->.
     solve_finz.
-    rewrite HpSome //=;clear HpSome.
-    rewrite (H2 2 ((of_pid p) ^+ 2)%f handle).
-    2: { apply finz_seq_lookup. rewrite H0. simpl. lia. solve_finz. }
-    2: { rewrite H0 /serialized_transaction_descriptor. by list_simplifier. }
+    rewrite (H1 2 ((of_pid p) ^+ 2)%f handle).
+    2: { apply finz_seq_lookup. rewrite H /=. lia. solve_finz. }
+    2: { rewrite H. by list_simplifier. }
     rewrite !decode_encode_vmid /=.
     reflexivity.
   Qed.
